add Liftable to buftxn specs

src/Helpers/BigOp.v
@@ -95,3 +95,23 @@ Proof.
   apply big_opL_gen_proper; auto.
   typeclasses eauto.
 Qed.
+
+Definition Conflicting {Σ L V} (P0 P1 : L -> V -> iProp Σ) :=
+  ∀ a0 v0 a1 v1,
+    P0 a0 v0 -∗ P1 a1 v1 -∗ ⌜ a0 ≠ a1 ⌝.
+
+Lemma big_sepM_disjoint_pred {Σ L V} {_ : EqDecision L} {_ : Countable L} (m0 m1 : gmap L V) (P0 P1 : L -> V -> iProp Σ) :
+  Conflicting P0 P1 ->
+  ( ( [∗ map] a↦v ∈ m0, P0 a v ) -∗
+    ( [∗ map] a↦v ∈ m1, P1 a v ) -∗
+    ⌜ m0 ##ₘ m1 ⌝ ).
+Proof.
+  iIntros (Hc) "H0 H1".
+  iIntros (i).
+  unfold option_relation.
+  destruct (m0 !! i) eqn:H0; destruct (m1 !! i) eqn:H1; try solve [ iPureIntro; auto ].
+  iDestruct (big_sepM_lookup with "H0") as "H0"; eauto.
+  iDestruct (big_sepM_lookup with "H1") as "H1"; eauto.
+  iDestruct (Hc with "H0 H1") as %Hcc.
+  congruence.
+Qed.
